dafny/Sort.dfy
@@ -1,16 +1,6 @@
 include "Blood.dfy"
 
-
-// use by
-predicate is_sorted(bloods: seq<Blood>, ascdesc: bool)
-requires forall i :: 0 <= i < |bloods| ==> bloods[i] != null;
-reads bloods;
-{
-    (ascdesc ==> (forall i, j: int :: 0 <= i < j < |bloods| ==> bloods[i].use_by <= bloods[j].use_by)) &&
-    (!ascdesc ==> (forall i, j: int :: 0 <= i < j < |bloods| ==> bloods[i].use_by >= bloods[j].use_by))
-}
-
-// multiset(a[..]) == multiset(old(a[..])) doesn't work, probably because of the type of the array
+// multiset(a[..]) == multiset(old(a[..])) doesn't work for array<Blood>, probably because of the type of the array
 // I have to make this function
 function toMultiset(input: array<Blood>): multiset<Blood>
 requires input != null;
@@ -22,109 +12,69 @@ reads input
     multiset(input[..])
 }
 
+/*
+method seq_to_array(bloods: seq<Blood>) returns (res: array<Blood>)
+requires forall i :: 0 <= i < |bloods| ==> bloods[i] != null;
+//ensures forall i :: 0 <= i < res.Length ==> res[i] != null;
+{
+    //res := new Blood[|bloods|] (i requires 0 <= i < |bloods| => (bloods[i]));
+    //res := new Blood[|bloods|];
+}
+*/
 
-predicate Sorted(a: array<Blood>, low:int, high:int)
-requires a != null // 1.9.7
-requires 0<=low<=high<=a.Length
-//requires forall i :: low <= i < high ==> a[i] != null;
-reads a
-reads set m | 0 <= m < a.Length :: a[m]
+predicate sorted_useby(bloods: array<Blood>, low:int, high:int)
+requires bloods != null 
+requires 0 <= low <= high <= bloods.Length
+requires forall i :: low <= i < high ==> bloods[i] != null;
+reads bloods
+reads set m | 0 <= m < bloods.Length :: bloods[m]
 { 
-    //forall i :: low <= i < high ==> a[i] != null && (forall j,k:: low<=j<k<high ==> a[j].use_by <= a[k].use_by)
-    true
+    forall i,j: int :: low <= i < j < high ==> bloods[i].use_by <= bloods[j].use_by
 }
 
 
-
-method InsertionSortSwap(bloods: array<Blood>)
-requires bloods != null // 1.9.7
+// verifies BloodFilter.py::sort_blood_by_useby_asc(bloods: list)
+method sort_blood_by_useby_asc(bloods: array<Blood>)
+requires bloods != null;
 requires forall i :: 0 <= i < bloods.Length ==> bloods[i] != null;
-ensures Sorted(bloods, 0, bloods.Length);
 ensures forall i :: 0 <= i < bloods.Length ==> bloods[i] != null;
+ensures sorted_useby(bloods, 0, bloods.Length);
 ensures toMultiset(bloods) == toMultiset(old(bloods));
 modifies bloods;
 {
     assert forall i :: 0 <= i < old(bloods).Length ==> old(bloods)[i] != null;
     assert toMultiset(bloods) == toMultiset(old(bloods));
-    var sorted_tail:=0;
+    var sorted_tail := 0;
+
     while (sorted_tail < bloods.Length)
+    decreases bloods.Length - sorted_tail;
     invariant 0 <= sorted_tail <= bloods.Length;
     //invariant forall i :: 0 <= i < sorted_tail ==> a[i] != null;
     invariant forall i :: 0 <= i < bloods.Length ==> bloods[i] != null;
     invariant toMultiset(bloods) == toMultiset(old(bloods));
-    invariant Sorted(bloods, 0, sorted_tail);
+    invariant sorted_useby(bloods, 0, sorted_tail);
     {
-        var down := sorted_tail; // the next unsorted element
-        while (down >= 1 && bloods[down - 1].use_by > bloods[down].use_by)
-        invariant 0 <= down <= sorted_tail;
-        //invariant forall i :: 0 <= i < down ==> a[i] != null;
-        //invariant forall i :: down <= i < sorted_tail ==> a[i] != null;
+        var to_swap := sorted_tail;
+        while (to_swap >= 1 && bloods[to_swap - 1].use_by > bloods[to_swap].use_by)
+        decreases to_swap;
+        invariant 0 <= to_swap <= sorted_tail;
+        //invariant forall i :: 0 <= i < to_swap ==> a[i] != null;
+        //invariant forall i :: to_swap <= i < sorted_tail ==> a[i] != null;
         invariant forall i :: 0 <= i < bloods.Length ==> bloods[i] != null;
         invariant toMultiset(bloods) == toMultiset(old(bloods));
-        //invariant forall i,j:: (0<=i<j<=sorted_tail && j!=down) ==> a[i].use_by <= a[j].use_by;
+        invariant forall i, j :: (0 <= i < j <= sorted_tail && j != to_swap) ==> bloods[i].use_by <= bloods[j].use_by;
         {
-            bloods[down - 1], bloods[down] := bloods[down], bloods[down - 1];
-            down := down-1;
+            bloods[to_swap - 1], bloods[to_swap] := bloods[to_swap], bloods[to_swap - 1];
+            to_swap := to_swap-1;
         }
         assert forall i :: 0 <= i <= sorted_tail ==> bloods[i] != null;
-        //assert down == 0 ==> a[down - 1].use_by => a[down].use_by;
+        //assert to_swap == 0 ==> a[to_swap - 1].use_by => a[to_swap].use_by;
         sorted_tail := sorted_tail + 1;
         assert forall i :: 0 <= i < sorted_tail ==> bloods[i] != null;
     }
     assert forall i :: 0 <= i < bloods.Length ==> bloods[i] != null;
     assert toMultiset(bloods) == toMultiset(old(bloods));
 }
-
-
-
-
-/*
-predicate Sorted1(a: array<Blood>, low:int, high:int)
-requires 0<=low<=high<=a.Length
-//requires forall i :: low <= i < high ==> a[i] != null;
-reads a
-reads set m | 0 <= m < a.Length :: a[m]
-{ 
-    forall j,k:: low<=j<k<high ==> a[j].use_by <= a[k].use_by
-    //true
-}
-
-
-
-method InsertionSortSwap1(a: array<Blood>)
-//requires a.Length > 1
-// requires forall i :: 0 <= i < a.Length ==> a[i] != null;
-ensures Sorted1(a, 0, a.Length);
-ensures toMultiset(a[..]) == toMultiset(old(a[..]));
-modifies a;
-{
-    var sorted_tail := 0;
-    while (sorted_tail < a.Length)
-    decreases a.Length - sorted_tail;
-    invariant 0 <= sorted_tail <= a.Length;
-    invariant toMultiset(a[..]) == toMultiset(old(a[..]));
-    invariant Sorted1(a, 0, sorted_tail);
-    {
-        var down := sorted_tail; // the next unordered element
-        while (down >= 1 && a[down-1].use_by > a[down].use_by)
-        decreases down;
-        invariant 0 <= down <= sorted_tail;
-        invariant toMultiset(a[..]) == toMultiset(old(a[..]));
-        // invariant forall i :: down <= i < sorted_tail ==> a[i] != null;
-        invariant forall i,j:: (0<=i<j<=sorted_tail && j!=down) ==> a[i].use_by <= a[j].use_by;
-        {
-            a[down-1], a[down] := a[down], a[down-1];
-            down:=down-1;
-        }
-        //assert down == 0 ==> a[down] != null;
-        sorted_tail := sorted_tail + 1;
-    }
-}
-
-
-*/
-
-
 
 method Main() {
     // this shows dafny has reference semantics
